Don't quote functor arguments (WIP)

theories/Template/QuoteGround/Init.v
@@ -2,12 +2,24 @@ From MetaCoq.Template Require Import MonadBasicAst MonadAst All utils.
 Require Import Coq.Lists.List.
 Import ListNotations.
 
+Local Set Primitive Projections.
 Local Open Scope bs.
 Import MCMonadNotation.
 
 Class quotation_of {T} (t : T) := quoted_term_of : Ast.term.
 Class ground_quotable T := quote_ground : forall t : T, quotation_of t.
+Class inductive_quotation_of {T} (t : T)
+  := { qinductive : inductive
+     ; qinst : Instance.t
+     ; qquotation : quotation_of t := tInd qinductive qinst }.
 Class debug_opt := debug : bool.
+Class cls_is_true (b : bool) := is_truev : is_true b.
+Definition default_inductive_quotation_of {T} {t : T} (qt : quotation_of t) (pf : cls_is_true match qt with tInd _ _ => true | _ => false end)
+  : inductive_quotation_of t
+  := match qt return cls_is_true match qt with tInd _ _ => true | _ => false end -> _ with
+     | tInd ind u => fun _ => @Build_inductive_quotation_of T t ind u
+     | _ => fun pf : false = true => match diff_false_true pf with end
+     end pf.
 
 (* returns true if a modpath is suitable for quotation, i.e., does not mention functor-bound arguments *)
 Fixpoint modpath_is_absolute (mp : modpath) : bool
@@ -16,69 +28,172 @@ Fixpoint modpath_is_absolute (mp : modpath) : bool
      | MPbound _ _ _ => false
      | MPdot mp _ => modpath_is_absolute mp
      end.
+Definition kername_is_absolute (kn : kername) : bool
+  := modpath_is_absolute (fst kn).
+
 (* returns false iff a term is suitable for quotation at the top-level, i.e., returns true iff it mentions functor-bound arguments or is a local variable or evar *)
 Definition head_term_is_bound (t : term) : bool
   := match t with
-     | tConst (kn, _) _ => negb (modpath_is_absolute kn)
+     | tConst kn _
+     | tInd {| inductive_mind := kn |} _
+     | tConstruct {| inductive_mind := kn |} _ _
+     | tProj {| proj_ind := {| inductive_mind := kn |} |} _
+     | tCase {| ci_ind := {| inductive_mind := kn |} |} _ _ _
+       => negb (kername_is_absolute kn)
      | tVar _
      | tEvar _ _
        => true
      | _ => false
      end.
 
-Fixpoint replace_quotation_of' {debug : debug_opt} (qt : term) : TemplateMonad term.
+Definition replace_inductive_kn (t : inductive) (i : term) : option inductive
+  := match i with
+     | tInd ind _
+       => Some {| inductive_mind := ind.(inductive_mind) ; inductive_ind := t.(inductive_ind) |}
+     | _ => None
+     end.
+
+Definition replace_head_ind (t : term) (i : term) : option term
+  := match t with
+     | tInd ind u
+       => option_map (fun ind => tInd ind u) (replace_inductive_kn ind i)
+     | tConstruct ind idx u
+       => option_map (fun ind => tConstruct ind idx u) (replace_inductive_kn ind i)
+     | tProj (mkProjection ind npars arg) t
+       => option_map (fun ind => tProj (mkProjection ind npars arg) t) (replace_inductive_kn ind i)
+     | tCase (mk_case_info ind npar rel) ti discr branches
+       => option_map (fun ind => tCase (mk_case_info ind npar rel) ti discr branches ) (replace_inductive_kn ind i)
+     | _ => None
+     end.
+
+Fixpoint head (t : term) : term
+  := match t with
+     | tCast t _ _
+     | tApp t _
+       => head t
+     | _ => t
+     end.
+
+Definition infer_replace_head_ind {debug : debug_opt} (qt : term) : TemplateMonad (option term).
+Proof.
+  simple
+    refine (let try_replace_head_ind qt v :=
+              (* make sure it's not just a context variable *)
+              (qv <- tmQuote v;;
+               match qv with
+               | tVar _ => ((if debug then tmPrint ("context variable:", v, "for", qt) else tmReturn tt);; tmReturn None)
+               | _ => tmReturn (replace_head_ind qt v)
+               end) in
+            match qt with
+            | tConstruct ind _ u
+            | tCase {| ci_ind := ind |} {| puinst := u |} _ _
+              => (ind <- tmUnquote (tInd ind u);;
+                  let '(existT_typed_term _ ind) := ind in
+                  v <- (tmInferInstance None (quotation_of ind));;
+                  match v with
+                  | my_Some v => try_replace_head_ind qt v
+                  | my_None => (if debug then tmPrint (quotation_of ind) else tmReturn tt);; tmReturn None
+                  end)
+            | tProj proj t
+              => (t <- tmUnquote t;;
+                  let '(existT_typed_term ty _) := t in
+                  ty <- tmEval hnf ty;;
+                  ty <- tmQuote ty;;
+                  let ind := head ty in
+                  ind <- tmUnquote ind;;
+                  let '(existT_typed_term _ ind) := ind in
+                  v <- (tmInferInstance None (quotation_of ind));;
+                  match v with
+                  | my_Some v => try_replace_head_ind qt v
+                  | my_None => (if debug then tmPrint (qt, quotation_of ind) else tmReturn tt);; tmReturn None
+                  end)
+            | _ => tmReturn None
+            end);
+    exact _.
+Defined.
+
+Definition try_infer_replace_head_ind {debug : debug_opt} (qt : term) : TemplateMonad term
+  := if head_term_is_bound qt
+     then (qt' <- infer_replace_head_ind qt;;
+           match qt' with
+           | Some qt => tmReturn qt
+           | None => tmReturn qt
+           end)
+     else tmReturn qt.
+Export bytestring.
+Fixpoint replace_quotation_of' {debug : debug_opt} (do_top_inference : bool) (qt : term) : TemplateMonad term.
 Proof.
   specialize (replace_quotation_of' debug).
   simple
     refine
-    (let tmInferQuotation t
+    (let replace_quotation_of' := replace_quotation_of' true in
+     tmPrint (do_top_inference, qt);;
+     let tmTryInferQuotation t
        := (t <- tmUnquote t;;
            let '(existT_typed_term _ t) := t in
-           v <- (tmInferInstance None (quotation_of t));;
-           match v with
-           | my_Some v => tmReturn v
-           | my_None => (if debug then tmPrint (quotation_of t) else tmReturn tt);; tmFail "No typeclass instance"
+           v <- tmInferInstance None (quotation_of t);;
+           match v return TemplateMonad (option_instance Ast.term) with
+           | my_Some v => tmReturn (@my_Some _ v)
+           | my_None => (if debug then tmPrint (quotation_of t) else tmReturn tt);; tmReturn (@my_None _)
            end) in
+     let tmInferQuotation t
+       := (v <- tmTryInferQuotation t;;
+           match v return TemplateMonad Ast.term with
+           | my_Some v => tmReturn v
+           | my_None => tmFail "No typeclass instance"
+           end) in
+     let replaced
+       := match qt return TemplateMonad Ast.term with
+          | tRel _
+          | tSort _
+          | tConstruct _ _ _
+          | tInt _
+          | tFloat _
+          | tConst _ _
+          | tInd _ _
+            => ret qt
+          | tVar _
+            => if do_top_inference then tmInferQuotation qt else tmFail "Avoiding loops"
+          | tEvar ev args => args <- monad_map replace_quotation_of' args;; ret (tEvar ev args)
+          | tLambda na T M => T <- replace_quotation_of' T;; M <- replace_quotation_of' M;; ret (tLambda na T M)
+          | tApp u v => u <- replace_quotation_of' u;; v <- monad_map replace_quotation_of' v;; ret (mkApps u v)
+          | tProd na A B => A <- replace_quotation_of' A;; B <- replace_quotation_of' B;; ret (tProd na A B)
+          | tCast c kind ty => c <- replace_quotation_of' c;; ty <- replace_quotation_of' ty;; ret (tCast c kind ty)
+          | tLetIn na b ty b' => b <- replace_quotation_of' b;; ty <- replace_quotation_of' ty;; b' <- replace_quotation_of' b';; ret (tLetIn na b ty b')
+          | tProj p c => replace_quotation_of' c;; ret (tProj p c)
+          | tFix mfix idx =>
+              mfix' <- monad_map (monad_map_def (TM:=TypeInstance) replace_quotation_of' replace_quotation_of') mfix;;
+              ret (tFix mfix' idx)
+          | tCoFix mfix idx =>
+              mfix' <- monad_map (monad_map_def (TM:=TypeInstance) replace_quotation_of' replace_quotation_of') mfix;;
+              ret (tCoFix mfix' idx)
+          | tCase ind p c brs =>
+              p' <- monad_map_predicate (TM:=TypeInstance) ret replace_quotation_of' replace_quotation_of' p;;
+              brs' <- monad_map_branches (TM:=TypeInstance) replace_quotation_of' brs;;
+              c <- replace_quotation_of' c;;
+              ret (tCase ind p' c brs')
+          end in
      if head_term_is_bound qt
-     then tmInferQuotation qt
+     then
+       v <- (if do_top_inference then tmTryInferQuotation qt else tmReturn (@my_None _));;
+       match v with
+       | my_Some v => tmReturn v
+       | my_None
+         => qt' <- replaced;;
+            qt' <- infer_replace_head_ind qt';;
+            match qt' with
+            | Some v => tmReturn v
+            | None => tmFail "No typeclass instance nor replacement"
+            end
+       end
      else
-       match qt return TemplateMonad Ast.term with
-       | tRel _
-       | tSort _
-       | tConstruct _ _ _
-       | tInt _
-       | tFloat _
-       | tConst _ _
-       | tInd _ _
-         => ret qt
-       | tVar _
-         => tmInferQuotation qt
-       | tEvar ev args => args <- monad_map replace_quotation_of' args;; ret (tEvar ev args)
-       | tLambda na T M => T <- replace_quotation_of' T;; M <- replace_quotation_of' M;; ret (tLambda na T M)
-       | tApp u v => u <- replace_quotation_of' u;; v <- monad_map replace_quotation_of' v;; ret (mkApps u v)
-       | tProd na A B => A <- replace_quotation_of' A;; B <- replace_quotation_of' B;; ret (tProd na A B)
-       | tCast c kind ty => c <- replace_quotation_of' c;; ty <- replace_quotation_of' ty;; ret (tCast c kind ty)
-       | tLetIn na b ty b' => b <- replace_quotation_of' b;; ty <- replace_quotation_of' ty;; b' <- replace_quotation_of' b';; ret (tLetIn na b ty b')
-       | tProj p c => replace_quotation_of' c;; ret (tProj p c)
-       | tFix mfix idx =>
-           mfix' <- monad_map (monad_map_def (TM:=TypeInstance) replace_quotation_of' replace_quotation_of') mfix;;
-           ret (tFix mfix' idx)
-       | tCoFix mfix idx =>
-           mfix' <- monad_map (monad_map_def (TM:=TypeInstance) replace_quotation_of' replace_quotation_of') mfix;;
-           ret (tCoFix mfix' idx)
-       | tCase ind p c brs =>
-           p' <- monad_map_predicate (TM:=TypeInstance) ret replace_quotation_of' replace_quotation_of' p;;
-           brs' <- monad_map_branches (TM:=TypeInstance) replace_quotation_of' brs;;
-           c <- replace_quotation_of' c;;
-           ret (tCase ind p' c brs')
-       end); exact _.
+       replaced);
+    try exact _.
 Defined.
 
 Definition replace_quotation_of {debug : debug_opt} {T} (t : T) : TemplateMonad term
   := qt <- tmQuote t;;
-     if head_term_is_bound qt
-     then tmFail "Avoiding loops"
-     else replace_quotation_of' qt.
+     replace_quotation_of' false qt.
 
 (** for fancier goals when we have [ground_quotable] for some subterms but not for subterms of those subterms *)
 Definition make_quotation_of {debug : debug_opt} {T} (t : T) : TemplateMonad (quotation_of t).
@@ -168,6 +283,19 @@ Module Export Instances.
    Hint Extern 1 (quotation_of _) => replace_quotation_of_goal () : typeclass_instances.
   #[export]
    Hint Extern 2 (quotation_of ?t) => make_quotation_of_goal () : typeclass_instances.
+  #[export] Hint Mode cls_is_true + : typeclass_instances.
+  #[export] Existing Instances qquotation | 10.
+  (* Hack around COQBUG(https://github.com/coq/coq/issues/16760) *)
+  #[export] Hint Extern 10 (@inductive_quotation_of ?T ?t) => simple notypeclasses refine (@default_inductive_quotation_of T t _ _) : typeclass_instances.
+  #[export] Hint Extern 10 (cls_is_true ?b)
+  => tryif is_evar b then refine (eq_refl true) else tryif has_evar b then fail else vm_compute; reflexivity
+       : typeclass_instances.
+  #[export] Hint Cut [
+      ( _ * )
+        qquotation
+        ( _ * )
+        qquotation
+    ] : typeclass_instances.
 End Instances.
 
 Module StrongerInstances.
